refactor: s/Env/AIG

LeanSAT/AIG/BoolExprCached.lean
@@ -1,62 +1,62 @@
 import LeanSAT.AIG.CachedGates
 import LeanSAT.AIG.CachedGatesLemmas
 
-namespace Env
+namespace AIG
 
 -- lines such as: ⟨ret, by dsimp [auxEntry, constEntry, ret] at *; omega⟩
 -- are slow in Meta.check
 -- TODO: minimize
 /--
 Turn a `BoolExprNat` into an AIG + entrypoint. Note that this version is meant for programming
-purposes. For proving use `Env.ofBoolExprNat` and equality theorems.
+purposes. For proving use `AIG.ofBoolExprNat` and equality theorems.
 -/
 def ofBoolExprNatCached (expr : BoolExpr Nat) : Entrypoint :=
-  go expr Env.empty |>.val
+  go expr AIG.empty |>.val
 where
-  go (expr : BoolExpr Nat) (env : Env) : { entry : Entrypoint // env.decls.size ≤ entry.env.decls.size } :=
+  go (expr : BoolExpr Nat) (aig : AIG) : { entry : Entrypoint // aig.decls.size ≤ entry.aig.decls.size } :=
     match expr with
-    | .literal var => ⟨env.mkAtomCached var, (by apply Env.mkAtomCached_le_size)⟩
-    | .const val => ⟨env.mkConstCached val, (by apply Env.mkConstCached_le_size)⟩
+    | .literal var => ⟨aig.mkAtomCached var, (by apply AIG.mkAtomCached_le_size)⟩
+    | .const val => ⟨aig.mkConstCached val, (by apply AIG.mkConstCached_le_size)⟩
     | .not expr =>
-      let ⟨exprEntry, _⟩ := go expr env
-      let ret := exprEntry.env.mkNotCached exprEntry.start exprEntry.inv
-      have := mkNotCached_le_size exprEntry.env exprEntry.start exprEntry.inv
+      let ⟨exprEntry, _⟩ := go expr aig
+      let ret := exprEntry.aig.mkNotCached exprEntry.start exprEntry.inv
+      have := mkNotCached_le_size exprEntry.aig exprEntry.start exprEntry.inv
       ⟨ret, by dsimp [ret] at *; omega⟩
     | .gate g lhs rhs =>
-      let ⟨lhsEntry, _⟩ := go lhs env
-      let ⟨rhsEntry, _⟩ := go rhs lhsEntry.env
-      have h1 : lhsEntry.start < Array.size rhsEntry.env.decls := by
+      let ⟨lhsEntry, _⟩ := go lhs aig
+      let ⟨rhsEntry, _⟩ := go rhs lhsEntry.aig
+      have h1 : lhsEntry.start < Array.size rhsEntry.aig.decls := by
         have := lhsEntry.inv
         omega
       match g with
       | .and =>
-        let ret := rhsEntry.env.mkAndCached lhsEntry.start rhsEntry.start h1 rhsEntry.inv
-        have := mkAndCached_le_size rhsEntry.env lhsEntry.start rhsEntry.start h1 rhsEntry.inv
+        let ret := rhsEntry.aig.mkAndCached lhsEntry.start rhsEntry.start h1 rhsEntry.inv
+        have := mkAndCached_le_size rhsEntry.aig lhsEntry.start rhsEntry.start h1 rhsEntry.inv
         ⟨ret, by dsimp [ret] at *; omega⟩
       | .or =>
-        let ret := rhsEntry.env.mkOrCached lhsEntry.start rhsEntry.start h1 rhsEntry.inv
-        have := mkOrCached_le_size rhsEntry.env lhsEntry.start rhsEntry.start h1 rhsEntry.inv
+        let ret := rhsEntry.aig.mkOrCached lhsEntry.start rhsEntry.start h1 rhsEntry.inv
+        have := mkOrCached_le_size rhsEntry.aig lhsEntry.start rhsEntry.start h1 rhsEntry.inv
         ⟨ret, by dsimp [ret] at *; omega⟩
       | .xor =>
-        let ret := rhsEntry.env.mkXorCached lhsEntry.start rhsEntry.start h1 rhsEntry.inv
-        have := mkXorCached_le_size rhsEntry.env lhsEntry.start rhsEntry.start h1 rhsEntry.inv
+        let ret := rhsEntry.aig.mkXorCached lhsEntry.start rhsEntry.start h1 rhsEntry.inv
+        have := mkXorCached_le_size rhsEntry.aig lhsEntry.start rhsEntry.start h1 rhsEntry.inv
         ⟨ret, by dsimp [ret] at *; omega⟩
       | .beq =>
-        let ret := rhsEntry.env.mkBEqCached lhsEntry.start rhsEntry.start h1 rhsEntry.inv
-        have := mkBEqCached_le_size rhsEntry.env lhsEntry.start rhsEntry.start h1 rhsEntry.inv
+        let ret := rhsEntry.aig.mkBEqCached lhsEntry.start rhsEntry.start h1 rhsEntry.inv
+        have := mkBEqCached_le_size rhsEntry.aig lhsEntry.start rhsEntry.start h1 rhsEntry.inv
         ⟨ret, by dsimp [ret] at *; omega⟩
       | .imp =>
-        let ret := rhsEntry.env.mkImpCached lhsEntry.start rhsEntry.start h1 rhsEntry.inv
-        have := mkImpCached_le_size rhsEntry.env lhsEntry.start rhsEntry.start h1 rhsEntry.inv
+        let ret := rhsEntry.aig.mkImpCached lhsEntry.start rhsEntry.start h1 rhsEntry.inv
+        have := mkImpCached_le_size rhsEntry.aig lhsEntry.start rhsEntry.start h1 rhsEntry.inv
         ⟨ret, by dsimp [ret] at *; omega⟩
 
-theorem ofBoolExprNatCached.go_decls_size_le (expr : BoolExpr Nat) (env : Env) :
-    env.decls.size ≤ (ofBoolExprNatCached.go expr env).val.env.decls.size := by
-  exact (ofBoolExprNatCached.go expr env).property
+theorem ofBoolExprNatCached.go_decls_size_le (expr : BoolExpr Nat) (aig : AIG) :
+    aig.decls.size ≤ (ofBoolExprNatCached.go expr aig).val.aig.decls.size := by
+  exact (ofBoolExprNatCached.go expr aig).property
 
-theorem ofBoolExprNatCached.go_decl_eq (idx) (env) (h : idx < env.decls.size) (hbounds) :
-    (ofBoolExprNatCached.go expr env).val.env.decls[idx]'hbounds = env.decls[idx] := by
-  induction expr generalizing env with
+theorem ofBoolExprNatCached.go_decl_eq (idx) (aig) (h : idx < aig.decls.size) (hbounds) :
+    (ofBoolExprNatCached.go expr aig).val.aig.decls[idx]'hbounds = aig.decls[idx] := by
+  induction expr generalizing aig with
   | const =>
     simp only [go]
     apply mkConstCached_decl_eq
@@ -65,15 +65,15 @@ theorem ofBoolExprNatCached.go_decl_eq (idx) (env) (h : idx < env.decls.size) (h
     apply mkAtomCached_decl_eq
   | not expr ih =>
     simp only [go]
-    have := go_decls_size_le expr env
-    specialize ih env (by omega) (by omega)
+    have := go_decls_size_le expr aig
+    specialize ih aig (by omega) (by omega)
     rw [mkNotCached_decl_eq]
     assumption
   | gate g lhs rhs lih rih =>
-    have := go_decls_size_le lhs env
-    have := go_decls_size_le rhs (go lhs env).val.env
-    specialize lih env (by omega) (by omega)
-    specialize rih (go lhs env).val.env (by omega) (by omega)
+    have := go_decls_size_le lhs aig
+    have := go_decls_size_le rhs (go lhs aig).val.aig
+    specialize lih aig (by omega) (by omega)
+    specialize rih (go lhs aig).val.aig (by omega) (by omega)
     cases g with
     | and =>
       simp only [go]
@@ -96,7 +96,7 @@ theorem ofBoolExprNatCached.go_decl_eq (idx) (env) (h : idx < env.decls.size) (h
       rw [mkImpCached_decl_eq]
       rw [rih, lih]
 
-theorem ofBoolExprNatCached.go_IsPrefix_env : IsPrefix env.decls (go expr env).val.env.decls := by
+theorem ofBoolExprNatCached.go_IsPrefix_aig : IsPrefix aig.decls (go expr aig).val.aig.decls := by
   apply IsPrefix.of
   . intro idx h
     apply ofBoolExprNatCached.go_decl_eq
@@ -104,16 +104,16 @@ theorem ofBoolExprNatCached.go_IsPrefix_env : IsPrefix env.decls (go expr env).v
 
 @[simp]
 theorem ofBoolExprNatCached.go_denote_entry (entry : Entrypoint) {h}:
-    ⟦(go expr entry.env).val.env, ⟨entry.start, h⟩, assign ⟧
+    ⟦(go expr entry.aig).val.aig, ⟨entry.start, h⟩, assign ⟧
       =
     ⟦entry, assign⟧ := by
-  apply denote.eq_of_env_eq
-  apply ofBoolExprNatCached.go_IsPrefix_env
+  apply denote.eq_of_aig_eq
+  apply ofBoolExprNatCached.go_IsPrefix_aig
 
 @[simp]
-theorem ofBoolExprNatCached.go_eval_eq_eval (expr : BoolExpr Nat) (env : Env) (assign) :
-    ⟦go expr env, assign⟧ = expr.eval assign := by
-  induction expr generalizing env with
+theorem ofBoolExprNatCached.go_eval_eq_eval (expr : BoolExpr Nat) (aig : AIG) (assign) :
+    ⟦go expr aig, assign⟧ = expr.eval assign := by
+  induction expr generalizing aig with
   | const => simp [go]
   | literal => simp [go]
   | not expr ih => simp [go, ih]
@@ -131,4 +131,4 @@ theorem ofBoolExprCached_unsat_iff : (ofBoolExprNatCached expr).unsat ↔ expr.u
     specialize h assign
     simpa using h
 
-end Env
+end AIG
