LeanSAT/AIG/LawfulOperator.lean
@@ -1,104 +1,104 @@
 import LeanSAT.AIG.Basic
 import LeanSAT.AIG.Lemmas
 
-namespace Env
+namespace AIG
 
-abbrev UnaryOperator := (gate : Nat) → (env : Env) → (gate < env.decls.size) → Entrypoint
+abbrev UnaryOperator := (gate : Nat) → (aig : AIG) → (gate < aig.decls.size) → Entrypoint
 
 class LawfulUnaryOperator (f : UnaryOperator) where
-  le_size : ∀ (env : Env) (gate : Nat) (hgate), env.decls.size ≤ (f gate env hgate).env.decls.size
-  decl_eq : ∀ (env : Env) (gate : Nat) (idx : Nat) (h1 : idx < env.decls.size) (hgate) (h2),
-    (f gate env hgate).env.decls[idx]'h2 = env.decls[idx]'h1
+  le_size : ∀ (aig : AIG) (gate : Nat) (hgate), aig.decls.size ≤ (f gate aig hgate).aig.decls.size
+  decl_eq : ∀ (aig : AIG) (gate : Nat) (idx : Nat) (h1 : idx < aig.decls.size) (hgate) (h2),
+    (f gate aig hgate).aig.decls[idx]'h2 = aig.decls[idx]'h1
 
 namespace LawfulUnaryOperator
 
 variable {f : UnaryOperator} [LawfulUnaryOperator f]
 
-theorem IsPrefix_env (env : Env) (gate : Nat) {hgate} :
-    IsPrefix env.decls (f gate env hgate).env.decls := by
+theorem IsPrefix_aig (aig : AIG) (gate : Nat) {hgate} :
+    IsPrefix aig.decls (f gate aig hgate).aig.decls := by
   apply IsPrefix.of
   . intro idx h
     apply decl_eq
   . apply le_size
 
 theorem lt_mkNotCached_size (entry : Entrypoint) (gate : Nat) (hgate) :
-    entry.start < (f gate entry.env hgate).env.decls.size := by
+    entry.start < (f gate entry.aig hgate).aig.decls.size := by
   have h1 := entry.inv
-  have h2 : entry.env.decls.size ≤ (f gate entry.env hgate).env.decls.size := by
+  have h2 : entry.aig.decls.size ≤ (f gate entry.aig hgate).aig.decls.size := by
     apply le_size
   omega
 
-theorem lt_size_of_lt_env_size (env : Env) (gate : Nat) (hgate) (h : x < env.decls.size)
-    : x < (f gate env hgate).env.decls.size := by
-  have := le_size (f := f) env gate hgate
+theorem lt_size_of_lt_aig_size (aig : AIG) (gate : Nat) (hgate) (h : x < aig.decls.size)
+    : x < (f gate aig hgate).aig.decls.size := by
+  have := le_size (f := f) aig gate hgate
   omega
 
-theorem le_size_of_le_env_size (env : Env) (gate : Nat) (hgate) (h : x ≤ env.decls.size)
-    : x ≤ (f gate env hgate).env.decls.size := by
-  have := le_size (f := f) env gate hgate
+theorem le_size_of_le_aig_size (aig : AIG) (gate : Nat) (hgate) (h : x ≤ aig.decls.size)
+    : x ≤ (f gate aig hgate).aig.decls.size := by
+  have := le_size (f := f) aig gate hgate
   omega
 
 @[simp]
 theorem denote_entry (entry : Entrypoint) {hgate} {h} :
-    ⟦(f gate entry.env hgate).env, ⟨entry.start, h⟩, assign ⟧
+    ⟦(f gate entry.aig hgate).aig, ⟨entry.start, h⟩, assign ⟧
       =
     ⟦entry, assign⟧ :=  by
-  apply denote.eq_of_env_eq
-  apply IsPrefix_env
+  apply denote.eq_of_aig_eq
+  apply IsPrefix_aig
 
-theorem denote_mem_prefix {env : Env} {hgate} (h) :
-    ⟦(f gate env hgate).env, ⟨start, by apply lt_size_of_lt_env_size; omega⟩, assign⟧
+theorem denote_mem_prefix {aig : AIG} {hgate} (h) :
+    ⟦(f gate aig hgate).aig, ⟨start, by apply lt_size_of_lt_aig_size; omega⟩, assign⟧
       =
-    ⟦env, ⟨start, h⟩, assign⟧ :=  by
-  rw [denote_entry ⟨env, start, h⟩]
+    ⟦aig, ⟨start, h⟩, assign⟧ :=  by
+  rw [denote_entry ⟨aig, start, h⟩]
 
 end LawfulUnaryOperator
 
-abbrev BinaryOperator := (lhs rhs : Nat) → (env : Env) → (lhs < env.decls.size) → (rhs < env.decls.size) → Entrypoint
+abbrev BinaryOperator := (lhs rhs : Nat) → (aig : AIG) → (lhs < aig.decls.size) → (rhs < aig.decls.size) → Entrypoint
 
 class LawfulBinaryOperator (f : BinaryOperator) where
-  le_size : ∀ (env : Env) (lhs rhs : Nat) (hl) (hr), env.decls.size ≤ (f lhs rhs env hl hr).env.decls.size
-  decl_eq : ∀ (env : Env) (lhs rhs : Nat) (idx : Nat) (h1 : idx < env.decls.size) (hl) (hr) (h2),
-    (f lhs rhs env hl hr).env.decls[idx]'h2 = env.decls[idx]'h1
+  le_size : ∀ (aig : AIG) (lhs rhs : Nat) (hl) (hr), aig.decls.size ≤ (f lhs rhs aig hl hr).aig.decls.size
+  decl_eq : ∀ (aig : AIG) (lhs rhs : Nat) (idx : Nat) (h1 : idx < aig.decls.size) (hl) (hr) (h2),
+    (f lhs rhs aig hl hr).aig.decls[idx]'h2 = aig.decls[idx]'h1
 
 namespace LawfulBinaryOperator
 
 variable {f : BinaryOperator} [LawfulBinaryOperator f]
 
-theorem IsPrefix_env (env : Env) (lhs rhs : Nat) {hl} {hr} :
-    IsPrefix env.decls (f lhs rhs env hl hr).env.decls := by
+theorem IsPrefix_aig (aig : AIG) (lhs rhs : Nat) {hl} {hr} :
+    IsPrefix aig.decls (f lhs rhs aig hl hr).aig.decls := by
   apply IsPrefix.of
   . intro idx h
     apply decl_eq
   . apply le_size
 
 theorem lt_size (entry : Entrypoint) (lhs hrs : Nat) (hl) (hr)
-    : entry.start < (f lhs rhs entry.env hl hr).env.decls.size := by
+    : entry.start < (f lhs rhs entry.aig hl hr).aig.decls.size := by
   have h1 := entry.inv
-  have h2 : entry.env.decls.size ≤ (f lhs rhs entry.env hl hr).env.decls.size := by
+  have h2 : entry.aig.decls.size ≤ (f lhs rhs entry.aig hl hr).aig.decls.size := by
     apply le_size
   omega
 
-theorem lt_size_of_lt_env_size (env : Env) (lhs rhs : Nat) (hl hr)
-    (h : x < env.decls.size)
-    : x < (f lhs rhs env hl hr).env.decls.size := by
-  have := le_size (f := f) env lhs rhs hl hr
+theorem lt_size_of_lt_aig_size (aig : AIG) (lhs rhs : Nat) (hl hr)
+    (h : x < aig.decls.size)
+    : x < (f lhs rhs aig hl hr).aig.decls.size := by
+  have := le_size (f := f) aig lhs rhs hl hr
   omega
 
 @[simp]
 theorem denote_entry (entry : Entrypoint) {hl} {hr} {h} :
-    ⟦(f lhs rhs entry.env hl hr).env, ⟨entry.start, h⟩, assign ⟧
+    ⟦(f lhs rhs entry.aig hl hr).aig, ⟨entry.start, h⟩, assign ⟧
       =
     ⟦entry, assign⟧ :=  by
-  apply denote.eq_of_env_eq
-  apply IsPrefix_env
+  apply denote.eq_of_aig_eq
+  apply IsPrefix_aig
 
-theorem denote_mem_prefix {env : Env} {hl} {hr} (h) :
-    ⟦(f lhs rhs env hl hr).env, ⟨start, (by apply lt_size_of_lt_env_size; omega)⟩, assign⟧
+theorem denote_mem_prefix {aig : AIG} {hl} {hr} (h) :
+    ⟦(f lhs rhs aig hl hr).aig, ⟨start, (by apply lt_size_of_lt_aig_size; omega)⟩, assign⟧
       =
-    ⟦env, ⟨start, h⟩, assign⟧ :=  by
-  rw [denote_entry ⟨env, start, h⟩]
+    ⟦aig, ⟨start, h⟩, assign⟧ :=  by
+  rw [denote_entry ⟨aig, start, h⟩]
 
 end LawfulBinaryOperator
 
-end Env
+end AIG
